Micro_C_Examples/C_Struct_Examples.thy
@@ -26,7 +26,7 @@ locale c_struct_verification_ctx =
     reference reference_types +
     ref_c_int: reference_allocatable reference_types _ _ _ _ _ _ _ c_int_prism +
     ref_c_point: reference_allocatable reference_types _ _ _ _ _ _ _ c_point_prism
-  for reference_types :: \<open>'s::{sepalg} \<Rightarrow> 'addr \<Rightarrow> 'gv \<Rightarrow> 'abort \<Rightarrow> 'i prompt \<Rightarrow>
+  for reference_types :: \<open>'s::{sepalg} \<Rightarrow> 'addr \<Rightarrow> 'gv \<Rightarrow> c_abort \<Rightarrow> 'i prompt \<Rightarrow>
         'o prompt_output \<Rightarrow> unit\<close>
   and c_int_prism :: \<open>('gv, c_int) prism\<close>
   and c_point_prism :: \<open>('gv, c_point) prism\<close>
@@ -67,9 +67,144 @@ definition c_swap_coords_contract :: \<open>('addr, 'gv, c_point) Global_Store.r
      in make_function_contract pre post\<close>
 ucincl_auto c_swap_coords_contract
 
+lemma c_point_x_focus_view [simp]:
+  shows \<open>focus_view (Abs_focus (make_focus_raw (\<lambda>s. Some (c_point_x s)) (\<lambda>y. update_c_point_x (\<lambda>_. y)))) pval = Some (c_point_x pval)\<close>
+proof -
+  have valid_via_modify: \<open>is_valid_focus (make_focus_raw_via_view_modify (\<lambda>s. Some (c_point_x s)) update_c_point_x)\<close>
+  proof (rule is_valid_focus_via_modifyI')
+    show \<open>is_valid_view_modify (\<lambda>s. Some (c_point_x s)) update_c_point_x\<close>
+      unfolding is_valid_view_modify_def
+    proof (intro conjI allI impI)
+      fix f s
+      show \<open>Some (c_point_x (update_c_point_x f s)) = map_option f (Some (c_point_x s))\<close>
+        by (cases s) simp
+    next
+      fix f s
+      assume eq: \<open>map_option f (Some (c_point_x s)) = Some (c_point_x s)\<close>
+      then have fx: \<open>f (c_point_x s) = c_point_x s\<close>
+        by simp
+      show \<open>update_c_point_x f s = s\<close>
+      proof (cases s)
+        case (make_c_point x1 x2)
+        from fx make_c_point have \<open>f x1 = x1\<close>
+          by simp
+        then show ?thesis
+          using make_c_point by (simp add: c_point.record_simps c_point.expand)
+      qed
+    next
+      fix f g s
+      show \<open>update_c_point_x f (update_c_point_x g s) = update_c_point_x (\<lambda>x. f (g x)) s\<close>
+        by (cases s) simp
+    qed
+  qed
+  then have valid: \<open>is_valid_focus (make_focus_raw (\<lambda>s. Some (c_point_x s)) (\<lambda>y. update_c_point_x (\<lambda>_. y)))\<close>
+    by (simp add: make_focus_raw_via_view_modify_def)
+  then show ?thesis
+    by (auto simp add: eq_onp_same_args focus_view.abs_eq Abs_focus_inverse)
+qed
+
+lemma c_point_y_focus_view [simp]:
+  shows \<open>focus_view (Abs_focus (make_focus_raw (\<lambda>s. Some (c_point_y s)) (\<lambda>y. update_c_point_y (\<lambda>_. y)))) pval = Some (c_point_y pval)\<close>
+proof -
+  have valid_via_modify: \<open>is_valid_focus (make_focus_raw_via_view_modify (\<lambda>s. Some (c_point_y s)) update_c_point_y)\<close>
+  proof (rule is_valid_focus_via_modifyI')
+    show \<open>is_valid_view_modify (\<lambda>s. Some (c_point_y s)) update_c_point_y\<close>
+      unfolding is_valid_view_modify_def
+    proof (intro conjI allI impI)
+      fix f s
+      show \<open>Some (c_point_y (update_c_point_y f s)) = map_option f (Some (c_point_y s))\<close>
+        by (cases s) simp
+    next
+      fix f s
+      assume eq: \<open>map_option f (Some (c_point_y s)) = Some (c_point_y s)\<close>
+      then have fy: \<open>f (c_point_y s) = c_point_y s\<close>
+        by simp
+      show \<open>update_c_point_y f s = s\<close>
+      proof (cases s)
+        case (make_c_point x1 x2)
+        from fy make_c_point have \<open>f x2 = x2\<close>
+          by simp
+        then show ?thesis
+          using make_c_point by (simp add: c_point.record_simps c_point.expand)
+      qed
+    next
+      fix f g s
+      show \<open>update_c_point_y f (update_c_point_y g s) = update_c_point_y (\<lambda>x. f (g x)) s\<close>
+        by (cases s) simp
+    qed
+  qed
+  then have valid: \<open>is_valid_focus (make_focus_raw (\<lambda>s. Some (c_point_y s)) (\<lambda>y. update_c_point_y (\<lambda>_. y)))\<close>
+    by (simp add: make_focus_raw_via_view_modify_def)
+  then show ?thesis
+    by (auto simp add: eq_onp_same_args focus_view.abs_eq Abs_focus_inverse)
+qed
+
+lemma c_point_x_lens_focus_view [simp]:
+  shows \<open>focus_view (Abs_focus (lens_to_focus_raw (make_lens_via_view_modify c_point_x update_c_point_x))) pval = Some (c_point_x pval)\<close>
+proof -
+  have valid_vm: \<open>is_valid_lens_view_modify c_point_x update_c_point_x\<close>
+    unfolding is_valid_lens_view_modify_def
+  proof (intro conjI allI impI)
+    fix f s
+    show \<open>c_point_x (update_c_point_x f s) = f (c_point_x s)\<close>
+      by (cases s) simp
+  next
+    fix f s
+    assume eq: \<open>f (c_point_x s) = c_point_x s\<close>
+    show \<open>update_c_point_x f s = s\<close>
+    proof (cases s)
+      case (make_c_point x1 x2)
+      from eq make_c_point have \<open>f x1 = x1\<close>
+        by simp
+      then show ?thesis
+        using make_c_point by (simp add: c_point.record_simps c_point.expand)
+    qed
+  next
+    fix f g s
+    show \<open>update_c_point_x f (update_c_point_x g s) = update_c_point_x (\<lambda>x. f (g x)) s\<close>
+      by (cases s) simp
+  qed
+  have valid: \<open>is_valid_lens (make_lens_via_view_modify c_point_x update_c_point_x)\<close>
+    by (rule is_valid_lens_via_modifyI'[OF valid_vm])
+  from lens_to_focus_raw_components'[OF valid] show ?thesis
+    by (simp add: make_lens_via_view_modify_components)
+qed
+
+lemma c_point_y_lens_focus_view [simp]:
+  shows \<open>focus_view (Abs_focus (lens_to_focus_raw (make_lens_via_view_modify c_point_y update_c_point_y))) pval = Some (c_point_y pval)\<close>
+proof -
+  have valid_vm: \<open>is_valid_lens_view_modify c_point_y update_c_point_y\<close>
+    unfolding is_valid_lens_view_modify_def
+  proof (intro conjI allI impI)
+    fix f s
+    show \<open>c_point_y (update_c_point_y f s) = f (c_point_y s)\<close>
+      by (cases s) simp
+  next
+    fix f s
+    assume eq: \<open>f (c_point_y s) = c_point_y s\<close>
+    show \<open>update_c_point_y f s = s\<close>
+    proof (cases s)
+      case (make_c_point x1 x2)
+      from eq make_c_point have \<open>f x2 = x2\<close>
+        by simp
+      then show ?thesis
+        using make_c_point by (simp add: c_point.record_simps c_point.expand)
+    qed
+  next
+    fix f g s
+    show \<open>update_c_point_y f (update_c_point_y g s) = update_c_point_y (\<lambda>x. f (g x)) s\<close>
+      by (cases s) simp
+  qed
+  have valid: \<open>is_valid_lens (make_lens_via_view_modify c_point_y update_c_point_y)\<close>
+    by (rule is_valid_lens_via_modifyI'[OF valid_vm])
+  from lens_to_focus_raw_components'[OF valid] show ?thesis
+    by (simp add: make_lens_via_view_modify_components)
+qed
+
 lemma c_swap_coords_spec:
   shows \<open>\<Gamma>; c_swap_coords pref \<Turnstile>\<^sub>F c_swap_coords_contract pref pg pval\<close>
-by (crush_boot f: c_swap_coords_def contract: c_swap_coords_contract_def) crush_base
+by (crush_boot f: c_swap_coords_def contract: c_swap_coords_contract_def)
+  (crush_base simp add: c_point.record_simps)
 
 end
 
