Micro_C_Parsing_Frontend/C_Translation_Smoke_Memory.thy
@@ -5,7 +5,7 @@ begin
 
 section \<open>Memory/Pointer Translation Smoke\<close>
 
-micro_c_translate \<open>
+micro_c_translate addr: nat \<open>
 void smoke_mem_swap(int *a, int *b) {
   int t = *a;
   *a = *b;
@@ -15,7 +15,7 @@ void smoke_mem_swap(int *a, int *b) {
 
 thm c_smoke_mem_swap_def
 
-micro_c_translate \<open>
+micro_c_translate addr: nat \<open>
 struct smoke_mem_point {
   int x;
   int y;
@@ -28,9 +28,8 @@ void smoke_mem_swap_fields(struct smoke_mem_point *p) {
 \<close>
 
 thm c_smoke_mem_swap_fields_def
-thm c_smoke_mem_point.record_simps
 
-micro_c_translate \<open>
+micro_c_translate addr: nat \<open>
 int smoke_mem_read_at(int *arr, int idx) {
   return arr[idx];
 }
@@ -38,7 +37,7 @@ int smoke_mem_read_at(int *arr, int idx) {
 
 thm c_smoke_mem_read_at_def
 
-micro_c_translate \<open>
+micro_c_translate addr: nat \<open>
 unsigned int smoke_mem_read_at_u(unsigned int *arr, unsigned int idx) {
   return arr[idx];
 }
@@ -46,7 +45,7 @@ unsigned int smoke_mem_read_at_u(unsigned int *arr, unsigned int idx) {
 
 thm c_smoke_mem_read_at_u_def
 
-micro_c_translate \<open>
+micro_c_translate addr: nat \<open>
 void smoke_mem_write_at(int *arr, int idx, int val) {
   arr[idx] = val;
 }
@@ -54,7 +53,7 @@ void smoke_mem_write_at(int *arr, int idx, int val) {
 
 thm c_smoke_mem_write_at_def
 
-micro_c_translate \<open>
+micro_c_translate addr: nat \<open>
 typedef unsigned char uint8_t;
 uint8_t smoke_mem_read_byte(uint8_t *buf, unsigned int idx) {
   return *(buf + idx);
@@ -63,7 +62,7 @@ uint8_t smoke_mem_read_byte(uint8_t *buf, unsigned int idx) {
 
 thm c_smoke_mem_read_byte_def
 
-micro_c_translate \<open>
+micro_c_translate addr: nat \<open>
 unsigned int smoke_mem_arr_param(unsigned int arr[], unsigned int i) {
   return arr[i];
 }
@@ -71,16 +70,16 @@ unsigned int smoke_mem_arr_param(unsigned int arr[], unsigned int i) {
 
 thm c_smoke_mem_arr_param_def
 
-micro_c_translate \<open>
+micro_c_translate addr: nat \<open>
 void smoke_mem_local_arr(void) {
-  unsigned int arr[] = {1, 2, 3};
+  unsigned int arr[3] = {1, 2, 3};
   unsigned int x = arr[1];
 }
 \<close>
 
 thm c_smoke_mem_local_arr_def
 
-micro_c_translate \<open>
+micro_c_translate addr: nat \<open>
 typedef unsigned char smoke_uint8_t;
 void smoke_mem_zero_init(void) {
   smoke_uint8_t t[4] = {0};
@@ -90,7 +89,7 @@ void smoke_mem_zero_init(void) {
 
 thm c_smoke_mem_zero_init_def
 
-micro_c_translate \<open>
+micro_c_translate addr: nat \<open>
 struct smoke_mem_point {
   int x;
   int y;
@@ -103,7 +102,7 @@ int smoke_mem_get_x(struct smoke_mem_point *p) {
 
 thm c_smoke_mem_get_x_def
 
-micro_c_translate \<open>
+micro_c_translate addr: nat \<open>
 unsigned int smoke_mem_inc_via_addr(void) {
   unsigned int x = 5;
   unsigned int *p = &x;
@@ -114,7 +113,7 @@ unsigned int smoke_mem_inc_via_addr(void) {
 
 thm c_smoke_mem_inc_via_addr_def
 
-micro_c_translate \<open>
+micro_c_translate addr: nat \<open>
 int smoke_mem_addr_of_index(int *arr, unsigned int idx) {
   int *p = &arr[idx];
   return *p;
@@ -123,7 +122,7 @@ int smoke_mem_addr_of_index(int *arr, unsigned int idx) {
 
 thm c_smoke_mem_addr_of_index_def
 
-micro_c_translate \<open>
+micro_c_translate addr: nat \<open>
 struct smoke_mem_holder {
   int vec[4];
 };
@@ -136,7 +135,35 @@ int smoke_mem_addr_of_struct_index(struct smoke_mem_holder *h, unsigned int i) {
 thm c_smoke_mem_addr_of_struct_index_def
 thm c_smoke_mem_holder.record_simps
 
-micro_c_translate \<open>
+micro_c_translate addr: nat \<open>
+struct smoke_mem_decay_holder {
+  int vec[4];
+};
+static int smoke_mem_sum2(int *p) {
+  return p[0] + p[1];
+}
+void smoke_mem_struct_array_decay_assign(struct smoke_mem_decay_holder *h, unsigned int i, int v) {
+  int *p;
+  p = h->vec;
+  p[i] = v;
+}
+int smoke_mem_struct_array_decay_init(struct smoke_mem_decay_holder *h, unsigned int i) {
+  int *p = h->vec;
+  return p[i];
+}
+int smoke_mem_struct_array_decay_pass(struct smoke_mem_decay_holder *h) {
+  int *p = h->vec;
+  return smoke_mem_sum2(p);
+}
+\<close>
+
+thm c_smoke_mem_sum2_def
+thm c_smoke_mem_struct_array_decay_assign_def
+thm c_smoke_mem_struct_array_decay_init_def
+thm c_smoke_mem_struct_array_decay_pass_def
+thm c_smoke_mem_decay_holder.record_simps
+
+micro_c_translate addr: nat \<open>
 const int smoke_mem_global_vals[3] = {1, 2, 3};
 int smoke_mem_read_global(unsigned int i) {
   return smoke_mem_global_vals[i];
